Tealeaves/Examples/VariadicLet/Terms.v
@@ -11,39 +11,42 @@ Export LN.Notations.
 #[local] Set Implicit Arguments.
 
 (** * Language definition *)
-(******************************************************************************)
-Inductive term (v : Type) :=
-| tvar : v -> term v
-| letin : list (term v) -> term v -> term v
-| app : term v -> term v -> term v.
+(**********************************************************************)
+Inductive term (v: Type) :=
+| tvar: v -> term v
+| abs: term v -> term v
+| letin: list (term v) -> term v -> term v
+| app: term v -> term v -> term v.
 
 #[export] Instance Return_Lam: Return term := tvar.
 
 Section term_mut_ind1.
 
   Variables
-    (v : Type)
-    (P : term v -> Prop).
+    (v: Type)
+    (P: term v -> Prop).
 
-  Hypotheses
-    (tvar_case : forall v, P (tvar v))
-      (letin_nil_case :  forall t, P t -> P (letin nil t))
-      (letin_cons_case : forall (u: term v) (l : list (term v)) (t: term v)
-                           (IHu: P u) (IHl: List.Forall P l)
-                           (IHt: P t), P (letin (u :: l) t))
-      (app_case : forall t: term v, P t -> forall u: term v, P u -> P (app t u)).
+  Context
+    (tvar_case: forall v, P (tvar v))
+    (abs_case: forall t: term v, P t -> P (abs t))
+    (letin_nil_case:  forall t, P t -> P (letin nil t))
+    (letin_cons_case: forall (u: term v) (l: list (term v)) (t: term v)
+    (IHu: P u) (IHl: List.Forall P l)
+    (IHt: P t), P (letin (u :: l) t))
+    (app_case: forall t: term v, P t -> forall u: term v, P u -> P (app t u)).
 
   Definition term_mut_ind: forall t, P t :=
     fix F t :=
       match t with
       | tvar v => tvar_case v
+      | abs body => @abs_case body (F body)
       | letin defs body =>
           match defs with
           | nil => @letin_nil_case body (F body)
           | cons u rest =>
               @letin_cons_case u rest body
                 (F u)
-                ((fix G l : List.Forall P l
+                ((fix G l: List.Forall P l
                   := match l with
                      | nil =>
                          List.Forall_nil P
@@ -58,7 +61,7 @@ Section term_mut_ind1.
 
 End term_mut_ind1.
 
-Lemma Forall_compat_list: forall (A: Type) (l : list A) (P: A -> Prop),
+Lemma Forall_compat_list: forall (A: Type) (l: list A) (P: A -> Prop),
     List.Forall P l <-> Forall_List P l.
 Proof.
   intros.
@@ -78,22 +81,24 @@ Qed.
 Section term_mut_ind2.
 
   Variables
-    (v : Type)
-    (P : term v -> Prop).
+    (v: Type)
+    (P: term v -> Prop).
 
   Hypotheses
-    (tvar_case : forall v, P (tvar v))
-    (letin_case : forall (defs: list (term v))
+    (tvar_case: forall v, P (tvar v))
+    (abs_case: forall t: term v, P t -> P (abs t))
+    (letin_case: forall (defs: list (term v))
                       (body: term v)
-                      (IHdefs: forall (t : term v), t ∈ defs -> P t)
+                      (IHdefs: forall (t: term v), t ∈ defs -> P t)
                       (IHbody: P body),
           P (letin defs body))
-    (app_case : forall t: term v, P t -> forall u: term v, P u -> P (app t u)).
+    (app_case: forall t: term v, P t -> forall u: term v, P u -> P (app t u)).
 
   Definition term_mut_ind2: forall t, P t.
   Proof.
     intros.
     induction t using term_mut_ind.
+    - auto.
     - auto.
     - apply letin_case.
       + inversion 1.
